type vs wf

CFG.thy
@@ -4,64 +4,44 @@ begin
 
 section \<open>Adjusted content from AFP/LocalLexing\<close>
 
-type_synonym 'a rule = "'a \<times> 'a list"
+datatype ('a, 'b) symbol = T 'a | NT 'b
 
-type_synonym 'a rules = "'a rule list"
+type_synonym ('a, 'b) rule = "('a, 'b) symbol \<times> ('a, 'b) symbol list"
 
-type_synonym 'a sentence = "'a list"
+type_synonym ('a, 'b) sentence = "('a, 'b) symbol list"
 
-datatype 'a cfg = 
-  CFG (\<NN> : "'a list") (\<TT> : "'a list") (\<RR> : "'a rules") (\<SS> : "'a")
+datatype ('a, 'b) cfg =
+   CFG (\<RR> : "('a, 'b) rule list") (\<SS> : "('a, 'b) symbol")
 
-definition disjunct_symbols :: "'a cfg \<Rightarrow> bool" where
-  "disjunct_symbols \<G> \<equiv> set (\<NN> \<G>) \<inter> set (\<TT> \<G>) = {}"
+definition wf_\<G> :: "('a, 'b) cfg \<Rightarrow> bool" where
+  "wf_\<G> \<G> \<equiv> distinct (\<RR> \<G>) \<and> (\<forall>N \<alpha>. (N, \<alpha>) \<in> set (\<RR> \<G>) \<longrightarrow> (\<exists>b. N = NT b)) \<and> (\<exists>b. \<SS> \<G> = NT b)"
 
-definition valid_startsymbol :: "'a cfg \<Rightarrow> bool" where
-  "valid_startsymbol \<G> \<equiv> \<SS> \<G> \<in> set (\<NN> \<G>)"
+definition is_terminal :: "('a, 'b) symbol \<Rightarrow> bool" where
+  "is_terminal x \<equiv> \<exists>a. x = T a"
 
-definition valid_rules :: "'a cfg \<Rightarrow> bool" where
-  "valid_rules \<G> \<equiv> \<forall>(N, \<alpha>) \<in> set (\<RR> \<G>). N \<in> set (\<NN> \<G>) \<and> (\<forall>s \<in> set \<alpha>. s \<in> set (\<NN> \<G>) \<union> set (\<TT> \<G>))"
-
-definition distinct_rules :: "'a cfg \<Rightarrow> bool" where
-  "distinct_rules \<G> \<equiv> distinct (\<RR> \<G>)"
-
-definition wf_\<G> :: "'a cfg \<Rightarrow> bool" where
-  "wf_\<G> \<G> \<equiv> disjunct_symbols \<G> \<and> valid_startsymbol \<G> \<and> valid_rules \<G> \<and> distinct_rules \<G>"
-
-lemmas wf_\<G>_defs = wf_\<G>_def valid_rules_def valid_startsymbol_def disjunct_symbols_def distinct_rules_def
-
-definition is_terminal :: "'a cfg \<Rightarrow> 'a \<Rightarrow> bool" where
-  "is_terminal \<G> x \<equiv> x \<in> set (\<TT> \<G>)"
-
-definition is_nonterminal :: "'a cfg \<Rightarrow> 'a \<Rightarrow> bool" where
-  "is_nonterminal \<G> x \<equiv> x \<in> set (\<NN> \<G>)"
-
-definition is_symbol :: "'a cfg \<Rightarrow> 'a \<Rightarrow> bool" where
-  "is_symbol \<G> x \<equiv> is_terminal \<G> x \<or> is_nonterminal \<G> x"
-
-definition wf_sentence :: "'a cfg \<Rightarrow> 'a sentence \<Rightarrow> bool" where
-  "wf_sentence \<G> \<omega> \<equiv> \<forall>x \<in> set \<omega>. is_symbol \<G> x"
+definition is_nonterminal :: "('a, 'b) symbol \<Rightarrow> bool" where
+  "is_nonterminal x \<equiv> \<exists>b. x = NT b"
 
 lemma is_nonterminal_startsymbol:
-  "wf_\<G> \<G> \<Longrightarrow> is_nonterminal \<G> (\<SS> \<G>)"
-  by (simp add: is_nonterminal_def wf_\<G>_defs)
+  "wf_\<G> \<G> \<Longrightarrow> is_nonterminal (\<SS> \<G>)"
+  by (simp add: is_nonterminal_def wf_\<G>_def)
 
-definition is_word :: "'a cfg \<Rightarrow> 'a sentence \<Rightarrow> bool" where
-  "is_word \<G> \<omega> \<equiv> \<forall>x \<in> set \<omega>. is_terminal \<G> x"
+definition is_word :: "('a, 'b) sentence \<Rightarrow> bool" where
+  "is_word \<omega> \<equiv> \<forall>x \<in> set \<omega>. is_terminal x"
 
-definition derives1 :: "'a cfg \<Rightarrow> 'a sentence \<Rightarrow> 'a sentence \<Rightarrow> bool" where
+definition derives1 :: "('a, 'b) cfg \<Rightarrow> ('a, 'b) sentence \<Rightarrow> ('a, 'b) sentence \<Rightarrow> bool" where
   "derives1 \<G> u v \<equiv> \<exists> x y N \<alpha>. 
     u = x @ [N] @ y \<and>
     v = x @ \<alpha> @ y \<and>
     (N, \<alpha>) \<in> set (\<RR> \<G>)"  
 
-definition derivations1 :: "'a cfg \<Rightarrow> ('a sentence \<times> 'a sentence) set" where
+definition derivations1 :: "('a, 'b) cfg \<Rightarrow> (('a, 'b) sentence \<times> ('a, 'b) sentence) set" where
   "derivations1 \<G> \<equiv> { (u,v) | u v. derives1 \<G> u v }"
 
-definition derivations :: "'a cfg \<Rightarrow> ('a sentence \<times> 'a sentence) set" where 
+definition derivations :: "('a, 'b) cfg \<Rightarrow> (('a, 'b) sentence \<times> ('a, 'b) sentence) set" where 
   "derivations \<G> \<equiv> (derivations1 \<G>)^*"
 
-definition derives :: "'a cfg \<Rightarrow> 'a sentence \<Rightarrow> 'a sentence \<Rightarrow> bool" where
+definition derives :: "('a, 'b) cfg \<Rightarrow> ('a, 'b) sentence \<Rightarrow> ('a, 'b) sentence \<Rightarrow> bool" where
   "derives \<G> u v \<equiv> ((u, v) \<in> derivations \<G>)"
 
 end
