Earley_Parser.thy
@@ -8,32 +8,32 @@ section \<open>Earley parser\<close>
 
 subsection \<open>Pointer lemmas\<close>
 
-definition predicts :: "'a item \<Rightarrow> bool" where
+definition predicts :: "('a, 'b) item \<Rightarrow> bool" where
   "predicts x \<equiv> item_origin x = item_end x \<and> item_dot x = 0"
 
-definition scans :: "'a sentence \<Rightarrow> nat \<Rightarrow> 'a item \<Rightarrow> 'a item \<Rightarrow> bool" where
+definition scans :: "('a, 'b) sentence \<Rightarrow> nat \<Rightarrow> ('a, 'b) item \<Rightarrow> ('a, 'b) item \<Rightarrow> bool" where
   "scans \<omega> k x y \<equiv> y = inc_item x k \<and> (\<exists>a. next_symbol x = Some a \<and> \<omega>!(k-1) = a)"
 
-definition completes :: "nat \<Rightarrow> 'a item \<Rightarrow> 'a item \<Rightarrow> 'a item \<Rightarrow> bool" where
+definition completes :: "nat \<Rightarrow> ('a, 'b) item \<Rightarrow> ('a, 'b) item \<Rightarrow> ('a, 'b) item \<Rightarrow> bool" where
   "completes k x y z \<equiv> y = inc_item x k \<and> is_complete z \<and> item_origin z = item_end x \<and>
     (\<exists>N. next_symbol x = Some N \<and> N = item_rule_head z)"
 
-definition sound_null_ptr :: "'a entry \<Rightarrow> bool" where
+definition sound_null_ptr :: "('a, 'b) entry \<Rightarrow> bool" where
   "sound_null_ptr e \<equiv> (pointer e = Null \<longrightarrow> predicts (item e))"
 
-definition sound_pre_ptr :: "'a sentence \<Rightarrow> 'a bins \<Rightarrow> nat \<Rightarrow> 'a entry \<Rightarrow> bool" where
+definition sound_pre_ptr :: "('a, 'b) sentence \<Rightarrow> ('a, 'b) bins \<Rightarrow> nat \<Rightarrow> ('a, 'b) entry \<Rightarrow> bool" where
   "sound_pre_ptr \<omega> bs k e \<equiv> \<forall>pre. pointer e = Pre pre \<longrightarrow>
     k > 0 \<and> pre < length (bs!(k-1)) \<and> scans \<omega> k (item (bs!(k-1)!pre)) (item e)"
 
-definition sound_prered_ptr :: "'a bins \<Rightarrow> nat \<Rightarrow> 'a entry \<Rightarrow> bool" where
+definition sound_prered_ptr :: "('a, 'b) bins \<Rightarrow> nat \<Rightarrow> ('a, 'b) entry \<Rightarrow> bool" where
   "sound_prered_ptr bs k e \<equiv> \<forall>p ps k' pre red. pointer e = PreRed p ps \<and> (k', pre, red) \<in> set (p#ps) \<longrightarrow>
     k' < k \<and> pre < length (bs!k') \<and> red < length (bs!k) \<and> completes k (item (bs!k'!pre)) (item e) (item (bs!k!red))"
 
-definition sound_ptrs :: "'a sentence \<Rightarrow> 'a bins \<Rightarrow> bool" where
+definition sound_ptrs :: "('a, 'b) sentence \<Rightarrow> ('a, 'b) bins \<Rightarrow> bool" where
   "sound_ptrs \<omega> bs \<equiv> \<forall>k < length bs. \<forall>e \<in> set (bs!k).
     sound_null_ptr e \<and> sound_pre_ptr \<omega> bs k e \<and> sound_prered_ptr bs k e"
 
-definition mono_red_ptr :: "'a bins \<Rightarrow> bool" where
+definition mono_red_ptr :: "('a, 'b) bins \<Rightarrow> bool" where
   "mono_red_ptr bs \<equiv> \<forall>k < length bs. \<forall>i < length (bs!k).
     \<forall>k' pre red ps. pointer (bs!k!i) = PreRed (k', pre, red) ps \<longrightarrow> red < i"
 
@@ -545,42 +545,42 @@ lemma sound_mono_ptrs_Earley\<^sub>L:
 
 subsection \<open>Common Definitions\<close>
 
-datatype 'a tree =
-  Leaf 'a
-  | Branch 'a "'a tree list"
+datatype ('a, 'b) tree =
+  Leaf "('a, 'b) symbol"
+  | Branch "('a, 'b) symbol" "('a, 'b) tree list"
 
-fun yield_tree :: "'a tree \<Rightarrow> 'a sentence" where
+fun yield_tree :: "('a, 'b) tree \<Rightarrow> ('a, 'b) sentence" where
   "yield_tree (Leaf a) = [a]"
 | "yield_tree (Branch _ ts) = concat (map yield_tree ts)"
 
-fun root_tree :: "'a tree \<Rightarrow> 'a" where
+fun root_tree :: "('a, 'b) tree \<Rightarrow> ('a, 'b) symbol" where
   "root_tree (Leaf a) = a"
 | "root_tree (Branch N _) = N"
 
-fun wf_rule_tree :: "'a cfg \<Rightarrow> 'a tree \<Rightarrow> bool" where
+fun wf_rule_tree :: "('a, 'b) cfg \<Rightarrow> ('a, 'b) tree \<Rightarrow> bool" where
   "wf_rule_tree _ (Leaf a) \<longleftrightarrow> True"
 | "wf_rule_tree \<G> (Branch N ts) \<longleftrightarrow> (
     (\<exists>r \<in> set (\<RR> \<G>). N = rule_head r \<and> map root_tree ts = rule_body r) \<and>
     (\<forall>t \<in> set ts. wf_rule_tree \<G> t))"
 
-fun wf_item_tree :: "'a cfg \<Rightarrow> 'a item \<Rightarrow> 'a tree \<Rightarrow> bool" where
+fun wf_item_tree :: "('a, 'b) cfg \<Rightarrow> ('a, 'b) item \<Rightarrow> ('a, 'b) tree \<Rightarrow> bool" where
   "wf_item_tree \<G> _ (Leaf a) \<longleftrightarrow> True"
 | "wf_item_tree \<G> x (Branch N ts) \<longleftrightarrow> (
     N = item_rule_head x \<and> map root_tree ts = take (item_dot x) (item_rule_body x) \<and>
     (\<forall>t \<in> set ts. wf_rule_tree \<G> t))"
 
-definition wf_yield_tree :: "'a sentence \<Rightarrow> 'a item \<Rightarrow> 'a tree \<Rightarrow> bool" where
+definition wf_yield_tree :: "('a, 'b) sentence \<Rightarrow> ('a, 'b) item \<Rightarrow> ('a, 'b) tree \<Rightarrow> bool" where
   "wf_yield_tree \<omega> x t \<longleftrightarrow> yield_tree t = slice (item_origin x) (item_end x) \<omega>"
 
-datatype 'a forest =
-  FLeaf 'a
-  | FBranch 'a "'a forest list list"
+datatype ('a, 'b) forest =
+  FLeaf "('a, 'b) symbol"
+  | FBranch "('a, 'b) symbol" "('a, 'b) forest list list"
 
 fun combinations :: "'a list list \<Rightarrow> 'a list list" where
   "combinations [] = [[]]"
 | "combinations (xs#xss) = [ x#cs . x <- xs, cs <- combinations xss ]"
 
-fun trees :: "'a forest \<Rightarrow> 'a tree list" where
+fun trees :: "('a, 'b) forest \<Rightarrow> ('a, 'b) tree list" where
   "trees (FLeaf a) = [Leaf a]"
 | "trees (FBranch N fss) = (
     let tss = (map (\<lambda>fs. concat (map (\<lambda>f. trees f) fs)) fss) in
@@ -726,7 +726,7 @@ qed simp
 
 subsection \<open>Parse tree\<close>
 
-partial_function (option) build_tree' :: "'a bins \<Rightarrow> 'a sentence \<Rightarrow> nat \<Rightarrow> nat \<Rightarrow> 'a tree option" where
+partial_function (option) build_tree' :: "('a, 'b) bins \<Rightarrow> ('a, 'b) sentence \<Rightarrow> nat \<Rightarrow> nat \<Rightarrow> ('a, 'b) tree option" where
   "build_tree' bs \<omega> k i = (
     let e = bs!k!i in (
     case pointer e of
@@ -753,7 +753,7 @@ partial_function (option) build_tree' :: "'a bins \<Rightarrow> 'a sentence \<Ri
 
 declare build_tree'.simps [code]
 
-definition build_tree :: "'a cfg \<Rightarrow> 'a sentence \<Rightarrow> 'a bins \<Rightarrow> 'a tree option" where
+definition build_tree :: "('a, 'b) cfg \<Rightarrow> ('a, 'b) sentence \<Rightarrow> ('a, 'b) bins \<Rightarrow> ('a, 'b) tree option" where
   "build_tree \<G> \<omega> bs = (
     let k = length bs - 1 in (
     case filter_with_index (\<lambda>x. is_finished \<G> \<omega> x) (items (bs!k)) of
@@ -780,7 +780,7 @@ lemma build_tree'_simps[simp]:
    build_tree' bs \<omega> k i = Some (Branch N (ts @ [t]))"
   by (subst build_tree'.simps, simp)+
 
-definition wf_tree_input :: "('a bins \<times> 'a sentence \<times> nat \<times> nat) set" where
+definition wf_tree_input :: "(('a, 'b) bins \<times> ('a, 'b) sentence \<times> nat \<times> nat) set" where
   "wf_tree_input = {
     (bs, \<omega>, k, i) | bs \<omega> k i.
       sound_ptrs \<omega> bs \<and>
@@ -789,7 +789,7 @@ definition wf_tree_input :: "('a bins \<times> 'a sentence \<times> nat \<times>
       i < length (bs!k)
   }"
 
-fun build_tree'_measure :: "('a bins \<times> 'a sentence \<times> nat \<times> nat) \<Rightarrow> nat" where
+fun build_tree'_measure :: "(('a, 'b) bins \<times> ('a, 'b) sentence \<times> nat \<times> nat) \<Rightarrow> nat" where
   "build_tree'_measure (bs, \<omega>, k, i) = foldl (+) 0 (map length (take k bs)) + i"
 
 lemma wf_tree_input_pre:
@@ -1261,7 +1261,7 @@ corollary wf_rule_root_yield_tree_build_tree_Earley\<^sub>L:
     length_Earley\<^sub>L_bins length_bins_Init\<^sub>L by (metis nle_le)
 
 theorem correctness_build_tree_Earley\<^sub>L:
-  assumes "wf_\<G> \<G>" "is_word \<G> \<omega>" "nonempty_derives \<G>"
+  assumes "wf_\<G> \<G>" "is_word \<omega>" "nonempty_derives \<G>"
   shows "(\<exists>t. build_tree \<G> \<omega> (Earley\<^sub>L \<G> \<omega>) = Some t) \<longleftrightarrow> derives \<G> [\<SS> \<G>] \<omega>" (is "?L \<longleftrightarrow> ?R")
 proof standard
   assume *: ?L
@@ -1537,7 +1537,7 @@ proof (induction xs arbitrary: vs)
   qed
 qed simp
 
-partial_function (option) build_trees' :: "'a bins \<Rightarrow> 'a sentence \<Rightarrow> nat \<Rightarrow> nat \<Rightarrow> nat set \<Rightarrow> 'a forest list option" where
+partial_function (option) build_trees' :: "('a, 'b) bins \<Rightarrow> ('a, 'b) sentence \<Rightarrow> nat \<Rightarrow> nat \<Rightarrow> nat set \<Rightarrow> ('a, 'b) forest list option" where
   "build_trees' bs \<omega> k i I = (
     let e = bs!k!i in (
     case pointer e of
@@ -1570,7 +1570,7 @@ partial_function (option) build_trees' :: "'a bins \<Rightarrow> 'a sentence \<R
 
 declare build_trees'.simps [code]
 
-definition build_trees :: "'a cfg \<Rightarrow> 'a sentence \<Rightarrow> 'a bins \<Rightarrow> 'a forest list option" where
+definition build_trees :: "('a, 'b) cfg \<Rightarrow> ('a, 'b) sentence \<Rightarrow> ('a, 'b) bins \<Rightarrow> ('a, 'b) forest list option" where
   "build_trees \<G> \<omega> bs = (
     let k = length bs - 1 in
     let finished = filter_with_index (\<lambda>x. is_finished \<G> \<omega> x) (items (bs!k)) in
@@ -1584,7 +1584,7 @@ lemma build_forest'_simps[simp]:
     build_trees' bs \<omega> k i I = those (map (\<lambda>f. case f of FBranch N fss \<Rightarrow> Some (FBranch N (fss @ [[FLeaf (\<omega>!(k-1))]])) | _ \<Rightarrow> None) pres)"
   by (subst build_trees'.simps, simp)+
 
-definition wf_trees_input :: "('a bins \<times> 'a sentence \<times> nat \<times> nat \<times> nat set) set" where
+definition wf_trees_input :: "(('a, 'b) bins \<times> ('a, 'b) sentence \<times> nat \<times> nat \<times> nat set) set" where
   "wf_trees_input = {
     (bs, \<omega>, k, i, I) | bs \<omega> k i I.
       sound_ptrs \<omega> bs \<and>
@@ -1594,7 +1594,7 @@ definition wf_trees_input :: "('a bins \<times> 'a sentence \<times> nat \<times
       i \<in> I
   }"
 
-fun build_forest'_measure :: "('a bins \<times> 'a sentence \<times> nat \<times> nat \<times> nat set) \<Rightarrow> nat" where
+fun build_forest'_measure :: "(('a, 'b) bins \<times> ('a, 'b) sentence \<times> nat \<times> nat \<times> nat set) \<Rightarrow> nat" where
   "build_forest'_measure (bs, \<omega>, k, i, I) = foldl (+) 0 (map length (take (k+1) bs)) - card I"
 
 lemma wf_trees_input_pre:
@@ -2464,7 +2464,7 @@ corollary wf_rule_root_yield_tree_build_trees_Earley\<^sub>L:
   by (metis dual_order.eq_iff )
 
 theorem soundness_build_trees_Earley\<^sub>L:
-  assumes "wf_\<G> \<G>" "is_word \<G> \<omega>" "nonempty_derives \<G>"
+  assumes "wf_\<G> \<G>" "is_word \<omega>" "nonempty_derives \<G>"
   assumes "build_trees \<G> \<omega> (Earley\<^sub>L \<G> \<omega>) = Some fs" "f \<in> set fs" "t \<in> set (trees f)"
   shows "derives \<G> [\<SS> \<G>] \<omega>"
 proof -
